theories/Core/Soundness/Realizability.v
@@ -1,0 +1,357 @@
+From Coq Require Import Nat.
+
+From Mcltt Require Import Base LibTactics.
+From Mcltt.Core.Syntactic Require Import CtxSub SystemOpt Corollaries CoreInversions.
+From Mcltt.Core Require Import PER.
+From Mcltt.Core.Semantic Require Import Realizability Readback.
+From Mcltt.Core.Soundness Require Export LogicalRelation Weakening.
+Import Domain_Notations.
+
+Open Scope list_scope.
+
+Lemma wf_ctx_sub_ctx_lookup : forall n T Γ,
+    {{ #n : T ∈ Γ }} ->
+    forall Δ,
+      {{ ⊢ Δ ⊆ Γ}} ->
+      exists Δ1 T0 Δ2 T',
+        Δ = Δ1 ++ T0 :: Δ2 /\
+          n = length Δ1 /\
+          T' = iter (S n) (fun T => {{{T [ Wk ]}}}) T0 /\
+          {{ #n : T' ∈ Δ }} /\
+          {{ Δ ⊢ T' ⊆ T }}.
+Proof.
+  induction 1; intros; progressive_inversion.
+  - exists nil.
+    repeat eexists; mauto 4.
+  - edestruct IHctx_lookup as [Δ1 [? [? [? [? [? [? []]]]]]]]; eauto.
+    exists (A0 :: Δ1). subst.
+    repeat eexists; mauto 4.
+Qed.
+
+
+Lemma var_arith : forall Γ1 Γ2 (T : typ),
+    length (Γ1 ++ T :: Γ2) - length Γ2 - 1 = length Γ1.
+Proof.
+  intros.
+  rewrite List.app_length. simpl.
+  lia.
+Qed.
+
+Lemma var_weaken_gen : forall Δ σ Γ,
+    {{ Δ ⊢w σ : Γ }} ->
+    forall Γ1 Γ2 T,
+      Γ = Γ1 ++ T :: Γ2 ->
+      {{Δ ⊢ (# (length Γ1)) [σ] ≈ # (length Δ - length Γ2 - 1) : ~(iter (S (length Γ1)) (fun T => {{{T [ Wk ]}}}) T) [ σ ] }}.
+Proof.
+  induction 1; intros; subst; gen_presups.
+  - pose proof (app_ctx_vlookup _ _ _ _ HΔ eq_refl).
+    gen_presup H0.
+    clear_dups.
+    apply wf_sub_id_inversion in Hτ.
+    pose proof (wf_ctx_sub_length _ _ Hτ).
+    transitivity {{{#(length Γ1) [Id]}}}; [mauto 3 |].
+    rewrite H1, var_arith, H.
+    bulky_rewrite. mauto 3.
+  - pose proof (app_ctx_vlookup _ _ _ _ HΔ0 eq_refl).
+    pose proof (app_ctx_lookup Γ1 T0 Γ2 _ eq_refl).
+    gen_presup H2.
+    clear_dups.
+    assert {{ Δ', T ⊢s Wk : ~ (Γ1 ++ {{{ Γ2, T0 }}}) }} by mauto.
+    transitivity {{{#(length Γ1) [Wk ∘ τ]}}}; [mauto 3 |].
+    rewrite H1.
+    etransitivity; [eapply wf_exp_eq_sub_compose; mauto 3 |].
+    pose proof (wf_ctx_sub_length _ _ H0).
+
+    rewrite <- exp_eq_sub_compose_typ; mauto 2.
+    deepexec wf_ctx_sub_ctx_lookup ltac:(fun H => destruct H as [? [? [? [? [-> [? [-> []]]]]]]]).
+    repeat rewrite List.app_length in *.
+    rewrite H6 in *.
+    assert (length x1 = length Γ2) by (simpl in *; lia).
+    rewrite <- H9.
+
+    etransitivity.
+    + eapply wf_exp_eq_sub_cong; [ |mauto 3].
+      eapply wf_exp_eq_subtyp.
+      * eapply wf_exp_eq_var_weaken; [mauto 3|]; eauto.
+      * mauto 4.
+    + eapply wf_exp_eq_subtyp.
+      * eapply IHweakening with (Γ1 := T :: _).
+        reflexivity.
+      * eapply wf_subtyping_subst; [ |mauto 3].
+        simpl. eapply wf_subtyping_subst; mauto 3.
+Qed.
+
+Lemma var_glu_elem_bot : forall A i P El Γ T,
+    {{ DG A ∈ glu_univ_elem i ↘ P ↘ El }} ->
+    {{ Γ ⊢ T ® P }} ->
+    {{ Γ, T ⊢ #0 : T[Wk] ® ! (length Γ) ∈ glu_elem_bot i A }}.
+Proof.
+  intros. saturate_glu_info.
+  econstructor; mauto 4.
+  - admit.
+  - intros. progressive_inversion.
+    exact (var_weaken_gen _ _ _ H2 nil _ _ eq_refl).
+Admitted.
+
+#[local]
+ Hint Rewrite -> wf_sub_eq_extend_compose using mauto 4 : mcltt.
+
+Theorem realize_glu_univ_elem_gen : forall A i P El,
+    {{ DG A ∈ glu_univ_elem i ↘ P ↘ El }} ->
+    (forall Γ T R, {{ DF A ≈ A ∈ per_univ_elem i ↘ R }} ->
+              {{ Γ ⊢ T ® P }} ->
+              {{ Γ ⊢ T ® glu_typ_top i A }}) /\
+      (forall Γ t T c, {{ DG A ∈ glu_univ_elem i ↘ P ↘ El }} ->
+                  {{ Γ ⊢ t : T ® c ∈ glu_elem_bot i A }} ->
+                  {{ Γ ⊢ t : T ® ⇑ A c ∈ El }}) /\
+      (forall Γ t T a R, {{ DG A ∈ glu_univ_elem i ↘ P ↘ El }} ->
+                    {{ Γ ⊢ t : T ® a ∈ El }} ->
+                    {{ DF A ≈ A ∈ per_univ_elem i ↘ R }} ->
+                    {{ Dom a ≈ a ∈ R }} ->
+                    {{ Γ ⊢ t : T ® a ∈ glu_elem_top i A }}).
+Proof.
+  simpl. induction 1 using glu_univ_elem_ind.
+  all:split; [| split]; intros;
+    apply_equiv_left;
+    gen_presups;
+    try match_by_head1 per_univ_elem ltac:(fun H => pose proof (per_univ_then_per_top_typ H));
+    match_by_head glu_elem_bot ltac:(fun H => destruct H as []);
+    destruct_all.
+  - econstructor; eauto; intros.
+    progressive_inversion.
+    transitivity {{{Type@j [ σ ]}}}; mauto 4.
+  - handle_functional_glu_univ_elem.
+    match_by_head glu_univ_elem invert_glu_univ_elem.
+    clear_dups.
+    apply_equiv_left.
+    repeat split; eauto.
+    repeat eexists.
+    + glu_univ_elem_econstructor; eauto; reflexivity.
+    + simpl. repeat split.
+      * rewrite <- H5. trivial.
+      * intros.
+        saturate_weakening_escape.
+        rewrite <- wf_exp_eq_typ_sub; try eassumption.
+        rewrite <- H5.
+        firstorder.
+  - deepexec glu_univ_elem_per_univ ltac:(fun H => pose proof H).
+    firstorder.
+    specialize (H _ _ _ H10) as [? []].
+    econstructor; eauto.
+    + apply_equiv_left. trivial.
+    + mauto 2.
+    + intros.
+      saturate_weakening_escape.
+      deepexec H ltac:(fun H => destruct H).
+      progressive_invert H16.
+      deepexec H20 ltac:(fun H => pose proof H).
+      functional_read_rewrite_clear.
+      bulky_rewrite.
+
+  - econstructor; eauto; intros.
+    progressive_inversion.
+    transitivity {{{ℕ [ σ ]}}}; mauto 3.
+  - handle_functional_glu_univ_elem.
+    match_by_head glu_univ_elem invert_glu_univ_elem.
+    apply_equiv_left.
+    repeat split; eauto.
+    econstructor; trivial.
+
+    intros.
+    saturate_weakening_escape.
+    assert {{ Δ ⊢ T [σ] ≈ ℕ[σ] : Type @ i }} by mauto 3.
+    rewrite <- wf_exp_eq_nat_sub; try eassumption.
+    rewrite <- H10. firstorder.
+  - econstructor; eauto.
+    + rewrite H2. mauto 3.
+    + apply_equiv_left. trivial.
+    + mauto 2.
+    + intros.
+      saturate_weakening_escape.
+      bulky_rewrite.
+      mauto using glu_nat_readback.
+
+  - match_by_head pi_glu_typ_pred progressive_invert.
+    handle_per_univ_elem_irrel.
+    invert_per_univ_elem H6.
+    econstructor; eauto; intros.
+    + gen_presups. trivial.
+    + saturate_weakening_escape.
+      assert {{ Γ ⊢w Id : Γ }} by mauto 4.
+      pose proof (H13 _ _ H16).
+      specialize (H13 _ _ H19).
+      assert {{ Γ ⊢ IT[Id] ≈ IT : Type@i}} by mauto 3.
+      bulky_rewrite_in H13.
+      progressive_invert H17.
+      destruct (H9 _ _ _ H0 H13) as [].
+      bulky_rewrite.
+      simpl. apply wf_exp_eq_pi_cong'; [firstorder |].
+      pose proof (var_per_elem (length Δ) H0).
+      destruct_rel_mod_eval.
+      simplify_evals.
+      destruct (H2 _ ltac:(eassumption) _ ltac:(eassumption)) as [? []].
+      specialize (H10 _ _ _ _ ltac:(trivial) (var_glu_elem_bot _ _ _ _ _ _ ltac:(eassumption) ltac:(eassumption))).
+      autorewrite with mcltt in H10.
+      specialize (H14 {{{Δ, IT[σ]}}} {{{σ ∘ Wk}}} _ _ ltac:(mauto) ltac:(eassumption) ltac:(eassumption)).
+      specialize (H8 _ _ _ ltac:(eassumption) ltac:(eassumption)) as [].
+      etransitivity; [| eapply H30]; mauto 3.
+  - handle_functional_glu_univ_elem.
+    apply_equiv_left.
+    invert_glu_rel1.
+    econstructor; try eapply per_bot_then_per_elem; eauto.
+
+    intros.
+    saturate_weakening_escape.
+    saturate_glu_info.
+    match_by_head1 per_univ_elem invert_per_univ_elem.
+    destruct_rel_mod_eval.
+    simplify_evals.
+    eexists; repeat split; mauto 3.
+    eapply H2; eauto.
+    assert {{ Δ ⊢ t [σ] : M[σ] }} by mauto 3.
+    bulky_rewrite_in H24.
+    unshelve (econstructor; eauto).
+    + trivial.
+    + eassert {{ Δ ⊢ ~ (a_sub t σ) m' : ~_ }} by (eapply wf_app'; eassumption).
+      autorewrite with mcltt in H26.
+      trivial.
+    + mauto using domain_app_per.
+    + intros.
+      saturate_weakening_escape.
+      progressive_invert H27.
+      destruct (H15 _ _ _ _ _ ltac:(eassumption) ltac:(eassumption) ltac:(eassumption) equiv_b).
+      handle_functional_glu_univ_elem.
+      autorewrite with mcltt.
+
+      etransitivity.
+      * rewrite sub_decompose_q_typ; mauto 4.
+      * simpl.
+        rewrite <- sub_eq_q_sigma_id_extend; mauto 4.
+        rewrite <- exp_eq_sub_compose_typ; mauto 3;
+          [eapply wf_exp_eq_app_cong' |].
+        -- specialize (H12 _ {{{σ ∘ σ0}}} _ ltac:(mauto 3) ltac:(eassumption)).
+           rewrite wf_exp_eq_sub_compose with (M := t) in H12; mauto 3.
+           bulky_rewrite_in H12.
+        -- rewrite <- exp_eq_sub_compose_typ; mauto 3.
+        -- econstructor; mauto 3.
+           autorewrite with mcltt.
+           rewrite <- exp_eq_sub_compose_typ; mauto 3.
+
+  - handle_functional_glu_univ_elem.
+    handle_per_univ_elem_irrel.
+    pose proof H8.
+    invert_per_univ_elem H8.
+    econstructor; mauto 3.
+    + invert_glu_rel1. trivial.
+    + eapply glu_univ_elem_trm_typ; eauto.
+    + intros.
+      saturate_weakening_escape.
+      invert_glu_rel1. clear_dups.
+      progressive_invert H20.
+
+      assert {{ Γ ⊢w Id : Γ }} by mauto 4.
+      pose proof (H10 _ _ H24).
+      specialize (H10 _ _ H19).
+      assert {{ Γ ⊢ IT[Id] ≈ IT : Type@i}} by mauto 3.
+      bulky_rewrite_in H25.
+      destruct (H11 _ _ _ ltac:(eassumption) ltac:(eassumption)) as [].
+      specialize (H29 _ _ _ H19 H9).
+      rewrite H5 in *.
+      autorewrite with mcltt.
+      eassert {{ Δ ⊢ m[σ] : ~_ }} by (mauto 2).
+      autorewrite with mcltt in H30.
+      rewrite @wf_exp_eq_pi_eta' with (M := {{{m[σ]}}}); [| trivial].
+      cbn [nf_to_exp].
+      eapply wf_exp_eq_fn_cong'; eauto.
+
+      pose proof (var_per_elem (length Δ) H0).
+      destruct_rel_mod_eval.
+      simplify_evals.
+      destruct (H2 _ ltac:(eassumption) _ ltac:(eassumption)) as [? []].
+      specialize (H12 _ _ _ _ ltac:(trivial) (var_glu_elem_bot _ _ _ _ _ _ H H10)).
+      autorewrite with mcltt in H12.
+      specialize (H14 {{{Δ, IT[σ]}}} {{{σ ∘ Wk}}} _ _ ltac:(mauto) ltac:(eassumption) ltac:(eassumption)) as [? []].
+      apply_equiv_left.
+      destruct_rel_mod_app.
+      simplify_evals.
+      deepexec H1 ltac:(fun H => pose proof H).
+      specialize (H33 _ _ _ _ _ ltac:(eassumption) ltac:(eassumption) ltac:(eassumption) ltac:(eassumption)) as [].
+      specialize (H40 _ {{{Id}}} _ ltac:(mauto 3) ltac:(eassumption)).
+      do 2 (rewrite wf_exp_eq_sub_id in H40; mauto 4).
+      etransitivity; [|eassumption].
+      simpl.
+      assert {{ Δ, IT[σ] ⊢ # 0 : IT[σ ∘ Wk] }} by (rewrite <- exp_eq_sub_compose_typ; mauto 3).
+      rewrite <- sub_eq_q_sigma_id_extend; mauto 4.
+      rewrite <- exp_eq_sub_compose_typ; mauto 2.
+      2:eapply sub_q; mauto 4.
+      2:gen_presup H41; econstructor; mauto 3.
+      eapply wf_exp_eq_app_cong'; [| mauto 3].
+      symmetry.
+      rewrite <- wf_exp_eq_pi_sub; mauto 4.
+
+  - econstructor; eauto.
+    intros.
+    progressive_inversion.
+    firstorder.
+  - handle_functional_glu_univ_elem.
+    apply_equiv_left.
+    econstructor; eauto.
+  - handle_functional_glu_univ_elem.
+    invert_glu_rel1.
+    econstructor; eauto.
+    + invert_glu_rel1.
+      specialize (H7 (length Γ)) as [? []].
+      specialize (H3 (length Γ)) as [? []].
+      assert {{ Γ ⊢w Id : Γ }} by mauto.
+      clear_dups. progressive_inversion.
+      deepexec H6 ltac:(fun H => pose proof H).
+      autorewrite with mcltt in H;
+        gen_presups; mauto 3.
+    + intros s. destruct (H1 s) as [? []].
+      mauto.
+    + intros.
+    progressive_inversion.
+    specialize (H10 (length Δ)) as [? []].
+    firstorder.
+
+Qed.
+
+Corollary realize_glu_typ_top : forall A i P El,
+    {{ DG A ∈ glu_univ_elem i ↘ P ↘ El }} ->
+    forall Γ T,
+      {{ Γ ⊢ T ® P }} ->
+      {{ Γ ⊢ T ® glu_typ_top i A }}.
+Proof.
+  intros.
+  pose proof H.
+  eapply glu_univ_elem_per_univ in H.
+  simpl in *. destruct_all.
+  eapply realize_glu_univ_elem_gen; eauto.
+Qed.
+
+Theorem realize_glu_elem_bot : forall A i P El,
+    {{ DG A ∈ glu_univ_elem i ↘ P ↘ El }} ->
+    forall Γ t T c,
+      {{ Γ ⊢ t : T ® c ∈ glu_elem_bot i A }} ->
+      {{ Γ ⊢ t : T ® ⇑ A c ∈ El }}.
+Proof.
+  intros.
+  eapply realize_glu_univ_elem_gen; eauto.
+Qed.
+
+Theorem realize_glu_elem_top : forall A i P El,
+    {{ DG A ∈ glu_univ_elem i ↘ P ↘ El }} ->
+    forall Γ t T a,
+      {{ Γ ⊢ t : T ® a ∈ El }} ->
+      {{ Γ ⊢ t : T ® a ∈ glu_elem_top i A }}.
+Proof.
+  intros.
+  pose proof H.
+  eapply glu_univ_elem_per_univ in H.
+  simpl in *. destruct_all.
+  eapply realize_glu_univ_elem_gen; eauto.
+  eapply glu_univ_elem_per_elem; eauto.
+Qed.
+
+#[export]
+  Hint Resolve realize_glu_typ_top realize_glu_elem_top : mcltt.
