theories/Core/Syntactic/Corollaries.v
@@ -1,4 +1,4 @@
-From Coq Require Import Setoid.
+From Coq Require Import Setoid Nat.
 From Mcltt Require Import Base LibTactics CtxSub.
 From Mcltt.Core Require Export SystemOpt CoreInversions.
 Import Syntax_Notations.
@@ -26,10 +26,105 @@ Qed.
 #[export]
 Hint Resolve invert_sub_id : mcltt.
 
-Add Parametric Morphism i Γ Δ t (H : {{ Δ ⊢ t : Type@i }}) : (a_sub t)
-    with signature wf_sub_eq Γ Δ ==> wf_exp_eq Γ {{{ Type@i }}} as sub_typ_cong1.
+Add Parametric Morphism i Γ Δ : a_sub
+    with signature wf_exp_eq Δ {{{ Type@i }}} ==> wf_sub_eq Γ Δ ==> wf_exp_eq Γ {{{ Type@i }}} as sub_typ_cong.
 Proof.
   intros.
   gen_presups.
   mauto 4.
+Qed.
+
+Add Parametric Morphism Γ1 Γ2 Γ3 : a_compose
+    with signature wf_sub_eq Γ2 Γ3 ==> wf_sub_eq Γ1 Γ2 ==> wf_sub_eq Γ1 Γ3 as sub_compose_cong.
+Proof. mauto. Qed.
+
+Lemma wf_ctx_sub_length : forall Γ Δ,
+    {{ ⊢ Γ ⊆ Δ }} ->
+    length Γ = length Δ.
+Proof. induction 1; simpl; auto. Qed.
+
+Open Scope list_scope.
+
+Lemma app_ctx_lookup : forall Δ T Γ n,
+    length Δ = n ->
+    {{ #n : ~(iter (S n) (fun T => {{{T [ Wk ]}}}) T) ∈ ~(Δ ++ T :: Γ) }}.
+Proof.
+  induction Δ; intros; simpl in *; subst; mauto.
+Qed.
+
+Lemma ctx_lookup_functional : forall n T Γ,
+    {{ #n : T ∈ Γ }} ->
+    forall T',
+      {{ #n : T' ∈ Γ }} ->
+      T = T'.
+Proof.
+  induction 1; intros; progressive_inversion; eauto.
+  erewrite IHctx_lookup; eauto.
+Qed.
+
+Lemma app_ctx_vlookup : forall Δ T Γ n,
+    {{ ⊢ ~(Δ ++ T :: Γ) }} ->
+    length Δ = n ->
+    {{ ~(Δ ++ T :: Γ) ⊢ #n : ~(iter (S n) (fun T => {{{T [ Wk ]}}}) T) }}.
+Proof.
+  intros. econstructor; auto using app_ctx_lookup.
+Qed.
+
+Lemma sub_q_eq : forall Δ A i Γ σ σ',
+                   {{ Δ ⊢ A : Type@i }} ->
+                   {{ Γ ⊢s σ ≈ σ' : Δ }} ->
+                   {{ Γ, A[σ] ⊢s q σ ≈ q σ' : Δ, A }}.
+Proof.
+  intros. gen_presup H0.
+  econstructor; mauto 3.
+  - econstructor; mauto 4.
+  - rewrite <- exp_eq_sub_compose_typ; mauto 4.
+Qed.
+#[export]
+ Hint Resolve sub_q_eq : mcltt.
+
+Lemma wf_subtyping_subst_eq : forall Δ A B,
+    {{ Δ ⊢ A ⊆ B }} ->
+    forall Γ σ σ',
+      {{ Γ ⊢s σ ≈ σ' : Δ }} ->
+      {{ Γ ⊢ A [σ] ⊆ B[σ'] }}.
+Proof.
+  induction 1; intros * Hσσ'; gen_presup Hσσ'.
+  - econstructor. mauto 4.
+  - etransitivity; mauto 4.
+  - autorewrite with mcltt.
+    mauto 2.
+  - autorewrite with mcltt.
+    eapply wf_subtyp_pi'; mauto.
+Qed.
+
+
+Lemma wf_subtyping_subst : forall Δ A B,
+    {{ Δ ⊢ A ⊆ B }} ->
+    forall Γ σ,
+      {{ Γ ⊢s σ : Δ }} ->
+      {{ Γ ⊢ A [σ] ⊆ B[σ] }}.
+Proof.
+  intros; mauto 2 using wf_subtyping_subst_eq.
+Qed.
+#[export]
+ Hint Resolve wf_subtyping_subst_eq wf_subtyping_subst : mcltt.
+
+Lemma sub_decompose_q_typ : forall Γ S T i σ Δ Δ' τ t,
+  {{Γ, S ⊢ T : Type@i}} ->
+  {{Δ ⊢s σ : Γ}} ->
+  {{Δ' ⊢s τ : Δ}} ->
+  {{Δ' ⊢ t : S [ σ ] [ τ ]}} ->
+  {{Δ' ⊢ T [ σ ∘ τ ,, t ] ≈ T [ q σ ] [ τ ,, t ] : Type@i}}.
+Proof.
+  intros. gen_presups.
+  simpl. autorewrite with mcltt.
+  rewrite wf_sub_eq_extend_compose; mauto 3;
+    [| mauto
+    | rewrite <- exp_eq_sub_compose_typ; mauto 4].
+  eapply exp_eq_sub_cong_typ2'; [mauto 2 | mauto |].
+  eapply wf_sub_eq_extend_cong; eauto.
+  - rewrite wf_sub_eq_compose_assoc; mauto 3; mauto 4.
+    rewrite wf_sub_eq_p_extend; eauto; mauto 4.
+  - rewrite <- exp_eq_sub_compose_typ; mauto 4.
 Qed.
